# Formeln & Co.

--

$$ \int_{-\infty}^{\infty} e^{-x^2} dx = \sqrt{\pi} $$

--

$$ \exp(-xyz) \cdot \log(x^2 + y^2) + \frac{\sin(x^2) \cdot \cos(y)}{\sqrt{z^3 + 1}} $$

--

<div style="display: flex; justify-content: center; align-items: center;">
$$
\begin{aligned}
\int (2x^3 - 3x^2 + x - 5) \, dx &= \int 2x^3 \, dx - \int 3x^2 \, dx + \int x \, dx - \int 5 \, dx \\
&= \frac{2}{4}x^4 - \frac{3}{3}x^3 + \frac{1}{2}x^2 - 5x + C \\
&= \frac{1}{2}x^4 - x^3 + \frac{1}{2}x^2 - 5x + C
\end{aligned}
$$
</div>

--

```latex
\begin{aligned}
\int (2x^3 - 3x^2 + x - 5) \, dx &= \int 2x^3 \, dx - \int 3x^2 \, dx + \int x \, dx - \int 5 \, dx \\
&= \frac{2}{4}x^4 - \frac{3}{3}x^3 + \frac{1}{2}x^2 - 5x + C \\
&= \frac{1}{2}x^4 - x^3 + \frac{1}{2}x^2 - 5x + C
\end{aligned}
```
